harden wip

clightplus_examples/hardening/src/hardening.c
@@ -1,52 +1,25 @@
 #include <stdint.h>
 
-typedef uintptr_t __u64;
-
-uintptr_t swab(uintptr_t x) {
-  uintptr_t ret;
-  ret = ((__u64)(         
-        (((__u64)(x) & (__u64)0x00000000000000ffULL) << 56) | 
-        (((__u64)(x) & (__u64)0x000000000000ff00ULL) << 40) |
-        (((__u64)(x) & (__u64)0x0000000000ff0000ULL) << 24) |
-        (((__u64)(x) & (__u64)0x00000000ff000000ULL) <<  8) |
-        (((__u64)(x) & (__u64)0x000000ff00000000ULL) >>  8) |
-        (((__u64)(x) & (__u64)0x0000ff0000000000ULL) >> 24) |
-        (((__u64)(x) & (__u64)0x00ff000000000000ULL) >> 40) |
-        (((__u64)(x) & (__u64)0xff00000000000000ULL) >> 56)));
-  return ret;
-}
-/* #define swab(x) ((__u64)(                              \ */
-/*         (((__u64)(x) & (__u64)0x00000000000000ffULL) << 56) |        \ */
-/*         (((__u64)(x) & (__u64)0x000000000000ff00ULL) << 40) |        \ */
-/*         (((__u64)(x) & (__u64)0x0000000000ff0000ULL) << 24) |        \ */
-/*         (((__u64)(x) & (__u64)0x00000000ff000000ULL) <<  8) |        \ */
-/*         (((__u64)(x) & (__u64)0x000000ff00000000ULL) >>  8) |        \ */
-/*         (((__u64)(x) & (__u64)0x0000ff0000000000ULL) >> 24) |        \ */
-/*         (((__u64)(x) & (__u64)0x00ff000000000000ULL) >> 40) |        \ */
-/*         (((__u64)(x) & (__u64)0xff00000000000000ULL) >> 56))) */
-
-uintptr_t encode(uintptr_t key, void *ptr, uintptr_t ptr_addr) {
+uintptr_t encode(uintptr_t key, void *ptr) {
   uintptr_t encoded;
-  encoded = (uintptr_t)ptr ^ key ^ swab(ptr_addr);
+  encoded = (uintptr_t)ptr ^ key;
   return encoded;
 }
 
-void *decode(uintptr_t key, uintptr_t ptr, uintptr_t ptr_addr) {
+void *decode(uintptr_t key, uintptr_t ptr) {
   void *decoded;
-  decoded = (void *)(ptr ^ key ^ swab(ptr_addr));
+  decoded = (void *)(ptr ^ key);
   return decoded;
 }
 
-long bar(uintptr_t key, uintptr_t ptr, uintptr_t ptr_addr) {
-  long *q = decode(key, ptr, ptr_addr);
-  return *q;
-}
+/* long bar(uintptr_t key, uintptr_t ptr) { */
+/*   long *q = decode(key, ptr); */
+/*   return *q; */
+/* } */
 
-long foo(uintptr_t key, uintptr_t ptr_addr) {
-  long *p;
-  *p = 42;
-  uintptr_t qi = encode(key, p, ptr_addr);
-  long ret = bar(key, qi, ptr_addr);
-  return ret;
-}
-// *q == 42
+/* long foo(uintptr_t key, long *p) { */
+/*   *p = 42; */
+/*   uintptr_t qi = encode(key, p); */
+/*   long ret = bar(key, qi); */
+/*   return ret; */
+/* } */
