clightplus_examples/hardening/hardening01proof.v
@@ -1,0 +1,134 @@
+Require Import CoqlibCCR.
+Require Import Any.
+Require Import STS.
+Require Import Behavior.
+Require Import ModSem.
+Require Import SimModSem.
+Require Import PCM.
+Require Import HoareDef.
+Require Import STB.
+Require Import HTactics ProofMode.
+Require Import HSim IProofMode.
+Require Import ClightPlusSkel ClightPlusExprgen ClightPlusgen.
+Require Import ClightPlusMemRA ClightPlusMem0 ClightPlusMem1 ClightPlusMemAux.
+Require Import CProofMode CIProofMode.
+Require Import hardening.
+Require Import hardening0.
+Require Import hardening1.
+
+(* Require Import xorlist. *)
+(* Require Import xorlistall0. *)
+(* Require Import xorlist1. *)
+Require Import PtrofsArith.
+From Coq Require Import Program.
+From compcert Require Import Memory Clightdefs.
+
+
+Section LEMMA.
+
+  Lemma f_bind_ret_r E R A (s : A -> itree E R)
+    : (fun a => ` x : R <- (s a);; Ret x) = s.
+  Proof. apply func_ext. i. apply bind_ret_r. Qed.
+
+  Lemma decode_encode_ofs i : decode_val Mint64 (encode_val Mint64 (Vptrofs i)) = Vptrofs i.
+  Proof.
+    pose proof (decode_encode_val_general (Vptrofs i) Mint64 Mint64).
+    unfold Vptrofs in *. des_ifs.
+  Qed.
+
+  Lemma decode_encode_item i : decode_val Mint64 (encode_val Mint64 (Vlong i)) = Vlong i.
+  Proof. apply (decode_encode_val_general (Vlong i) Mint64 Mint64). Qed.
+
+  Lemma decode_encode_null : decode_val Mint64 (encode_val Mint64 Vnullptr) = Vnullptr.
+  Proof. rewrite (decode_encode_val_general Vnullptr Mint64 Mint64). et. Qed.
+
+  Lemma null_zero i : Vptrofs i = Vnullptr -> i = Ptrofs.zero.
+  Proof.
+    unfold Vptrofs, Vnullptr. des_ifs. i.
+    apply (f_equal (fun v: val => match v with Vlong i => i | _ => Int64.zero end)) in H.
+    rewrite <- (Ptrofs.of_int64_to_int64 Heq i). rewrite H. et.
+  Qed.
+
+  Context `{eventE -< eff}.
+
+  Lemma cast_ptrofs i : cast_to_ptr (Vptrofs i) = Ret (Vptrofs i).
+  Proof. des_ifs. Qed.
+
+  Lemma cast_long i : Archi.ptr64 = true -> cast_to_ptr (Vlong i) = Ret (Vlong i).
+  Proof. ss. Qed.
+
+End LEMMA.
+
+Section PROOF.
+
+  Import ClightPlusMem1.
+
+  Context `{@GRA.inG Mem.t Σ}.
+
+  Variable GlobalStb : Sk.t -> gname -> option fspec.
+  Hypothesis STBINCL : forall sk, stb_incl (to_stb hardeningStb) (GlobalStb sk).
+  Hypothesis MEMINCL : forall sk, stb_incl (to_stb MemStb) (GlobalStb sk).
+
+
+  Definition wf : _ -> Any.t * Any.t -> Prop :=
+    @mk_wf
+      _
+      unit
+      (fun _ st_src st_tgt => ⌜True⌝)%I.
+
+  Let mfsk : Sk.t := [("malloc", Gfun (F:=Clight.fundef) (V:=type) (Ctypes.External EF_malloc (Tcons tulong Tnil) (tptr tvoid) cc_default)); ("free", Gfun (Ctypes.External EF_free (Tcons (tptr tvoid) Tnil) tvoid cc_default))].
+
+  Section SIMFUNS.
+  Variable hardening_code : Clight.program.
+  (* Variable xormod : Mod.t. *)
+  (* Hypothesis VALID_link : xorlistall0._xor = Some xorlink. *)
+  (* Hypothesis VALID_comp : compile xorlink "xorlist" = Errors.OK xormod. *)
+  Let ce := Maps.PTree.elements (prog_comp_env hardening_code).
+
+  Variable sk: Sk.t.
+  (* TODO: How to encapsulate fuction info? *)
+  (* Hypothesis SKINCL1 : Sk.le (xormod.(Mod.sk)) sk. *)
+  Hypothesis SKINCL : Sk.le mfsk sk.
+  Hypothesis SKWF : Sk.wf sk.
+
+  Lemma encode :
+    sim_fnsem wf top2
+      ("encode", fun_to_tgt "hardening" (GlobalStb sk) (mk_pure encode_spec))
+      ("encode", cfunU (decomp_func sk ce f_encode)).
+  Proof.
+    Local Opaque encode_val.
+    Local Opaque cast_to_ptr.
+    eassert (_hardening = _).
+    { unfold _hardening. reflexivity. }
+    (* rewrite H0 in *. clear H0. *)
+    (* destruct Ctypes.link_build_composite_env. destruct a. *)
+    (* inversion VALID_link. clear VALID_link. subst. *)
+    (* clear a. simpl in ce. *)
+    econs; ss. red.
+
+    (* get_composite ce e. *)
+    dup SKINCL. rename SKINCL0 into SKINCLENV.
+    apply incl_incl_env in SKINCLENV.
+    unfold incl_env in SKINCLENV.
+    pose proof sk_incl_gd as SKINCLGD.
+
+    apply isim_fun_to_tgt; auto.
+    unfold f_encode. i; ss.
+    unfold decomp_func, function_entry_c. ss.
+
+    let H := fresh "HIDDEN" in
+    set (H := hide 1).
+    
+    iIntros "[INV PRE]". des_ifs_safe. ss.
+    iDestruct "PRE" as "[[% PRE] %]".
+    des. clarify. hred_r.
+
+    rename v into iptr, v0 into ptr.
+
+    unhide. hred_r. unhide. remove_tau. unhide. remove_tau.
+
+
+
+  End SIMFUNS.
+
+End Proof.
