clightplus_examples/hardening/hardening1.v
@@ -1,0 +1,91 @@
+Require Import CoqlibCCR.
+Require Import Skeleton.
+Require Import PCM.
+Require Import HoareDef.
+Require Import ProofMode.
+Require Import STB.
+Require Import Any.
+Require Import ModSem.
+Require Import ModSemE.
+Require Import ClightPlusMemRA.
+Require Import ClightPlusMem1.
+From compcert Require Export Ctypes Values AST Memdata Integers.
+
+Set Implicit Arguments.
+
+Section PROP.
+
+  Context `{@GRA.inG Mem.t Σ}.
+
+  (* Definition swab_func (v: val) : val := *)
+  (*   match v with *)
+  (*   | Vlong n => if Archi.ptr64 then Vlong n else Vundef *)
+  (*   | Vint n => if negb Archi.ptr64 then Vint n else Vundef *)
+  (*   | _ => Vundef *)
+  (*   end. *)
+
+End PROP.
+
+Section SPEC.
+
+  Context `{@GRA.inG Mem.t Σ}.
+
+  (* uintptr_t encode(uintptr_t key, void *ptr) { *)
+  (*   uintptr_t encoded; *)
+  (*   encoded = (uintptr_t)ptr ^ key; *)
+  (*   return encoded; *)
+  (* } *)
+
+  Definition encode_spec : fspec :=
+    (mk_simple
+      (fun '(key, ptr, m_ptr, tg, q, iptr) => (
+        (ord_pure 1%nat),
+        (fun varg => ⌜varg = [Vlong key; ptr]↑⌝
+                     ** live_(m_ptr,tg,q) ptr),
+        (fun vret => ⌜vret = (Val.xorl iptr (Vlong key))↑⌝
+                     ** live_(m_ptr,tg,q) ptr ** ptr (≃_ m_ptr) iptr)
+    )))%I.
+
+  (* void *decode(uintptr_t key, uintptr_t ptr) { *)
+  (*   void *decoded; *)
+  (*   decoded = (void *\) (ptr ^ key); *)
+  (*   return decoded; *)
+  (* } *)
+  
+  Definition decode_spec : fspec :=
+    (mk_simple
+      (fun '(key, ptr) => (
+        (ord_pure 1%nat),
+        (fun varg => ⌜varg = [Vlong key; (Vlong ptr)]↑⌝),
+        (fun vret => ⌜vret = (Val.xorl (Vlong ptr) (Vlong key))↑⌝)
+    )))%I.
+
+  (* sealed *)
+  Definition hardeningStb : list (gname * fspec).
+    eapply (Seal.sealing "stb").
+    apply [
+           ("encode", encode_spec);
+           ("decode", decode_spec)
+           (* ; *)
+           (* ("delete_hd", delete_hd_spec); *)
+           (* ("delete_tl", delete_tl_spec) *)
+           (* ("search", search_spec) *)
+           ].
+  Defined.
+
+End SPEC.
+
+Section SMOD.
+
+  Context `{@GRA.inG Mem.t Σ}.
+
+  Definition hardeningSbtb: list (gname * fspecbody) :=
+    [
+     ("encode", mk_pure encode_spec);
+     ("decode", mk_pure decode_spec)
+     (* ; *)
+     (* ("delete_hd", mk_pure delete_hd_spec); *)
+     (* ("delete_tl", mk_pure delete_tl_spec) *)
+     ].
+
+End SMOD.
